fix(init/meta/tactic): let by_cases handle elimination to Type

library/init/meta/interactive.lean
@@ -799,9 +799,9 @@ do e ← to_expr p, guard (alpha_eqv t e)
 meta def guard_target (p : parse texpr) : tactic unit :=
 do t ← target, guard_expr_eq t p
 
-meta def by_cases (q : parse texpr) : tactic unit :=
+meta def by_cases (q : parse texpr) (n : parse (tk "with" *> ident)?): tactic unit :=
 do p ← tactic.to_expr_strict q,
-   tactic.by_cases p
+   tactic.by_cases p (n.get_or_else `h)
 
 meta def by_contradiction : tactic unit :=
 tactic.by_contradiction >> return ()
