library/data/bitvec.lean
@@ -42,11 +42,9 @@ section shift
   bitvec.cong
     begin
       by_cases (i ≤ n),
-      { intro h,
-        note h₁ := sub_le n i,
+      { note h₁ := sub_le n i,
         rw [min_eq_right h], rw [min_eq_left h₁, -nat.add_sub_assoc h, add_comm, nat.add_sub_cancel] },
-      { intro h,
-        note h₁ := le_of_not_ge h,
+      { note h₁ := le_of_not_ge h,
         rw [min_eq_left h₁, sub_eq_zero_of_le h₁, min_zero_left, add_zero] }
     end $
     repeat fill (min n i) ++ₜ taken (n-i) x
